bounded frame length, close #1

src/Util/ByteVector.v
@@ -1,6 +1,7 @@
 From Coq Require Import Ascii NArith String Vector.
 Import VectorNotations.
 Open Scope string_scope.
+Open Scope N_scope.
 
 Definition ByteVector := Vector.t ascii.
 Definition ByteNil : ByteVector 0 := Vector.nil ascii.
@@ -17,10 +18,49 @@ Fixpoint from_string (s : string) : ByteVector (length s) :=
   | String b s' => b::from_string s'
   end.
 
-Fixpoint N_of_ByteVector_rec {n : nat} (acc : N) (v : ByteVector n) : N :=
+Fixpoint N_of_ByteVector {n : nat} (v : ByteVector n) : N :=
   match v with
-  | [] => acc
-  | a::v' => N_of_ByteVector_rec (N.shiftl acc 8 + N_of_ascii a) v'
+  | [] => 0
+  | a::v' =>
+    match n with
+    | O => 0                     (* unreachable *)
+    | S n' => N.shiftl_nat (N_of_ascii a) (n' * 8) + N_of_ByteVector v'
+    end
   end.
 
-Definition N_of_ByteVector {n : nat} : ByteVector n -> N := N_of_ByteVector_rec 0.
+Lemma ascii_upperbound' (a : ascii) : N_of_ascii a < 256.
+Proof with simpl; constructor.
+  destruct a as [b0 b1 b2 b3 b4 b5 b6 b7].
+  destruct b0;
+  destruct b1;
+  destruct b2;
+  destruct b3;
+  destruct b4;
+  destruct b5;
+  destruct b6;
+  destruct b7...
+Qed.
+
+Corollary ascii_upperbound (a : ascii) : N_of_ascii a <= 255.
+Proof with auto.
+  replace 255 with (N.pred 256)...
+  apply N.lt_le_pred.
+  apply ascii_upperbound'.
+Qed.
+
+Lemma ByteVector_upperbound : forall (n : nat) (v : ByteVector n), N_of_ByteVector v < N.shiftl_nat 1 (n * 8).
+Proof with simpl; auto.
+  induction v...
+  - constructor.
+  - repeat rewrite <- Nshiftl_equiv_nat in *.
+    repeat rewrite N.shiftl_mul_pow2 in *.
+    repeat rewrite N.double_mul.
+    replace (N.double (N.double (N.double (N.double (N.double (N.double (N.double (N.double 1)))))))) with (255 + 1).
+    + apply N.le_lt_trans with (m := 255 * 2 ^ N.of_nat (n * 8) + N_of_ByteVector v).
+      * apply N.add_le_mono_r.
+        apply N.mul_le_mono_r.
+        apply ascii_upperbound.
+      * rewrite N.mul_add_distr_r.
+        apply N.add_lt_mono_l...
+    + reflexivity.
+Qed.
